ConNF.lean
@@ -22,6 +22,8 @@ import ConNF.Counting.Conclusions
 import ConNF.Counting.CountSupportOrbit
 import ConNF.Counting.Recode
 import ConNF.Counting.Twist
+import ConNF.External.Basic
+import ConNF.External.WellOrder
 import ConNF.FOA.BaseAction
 import ConNF.FOA.BaseApprox
 import ConNF.FOA.Coherent
