ConNF/External/Basic.lean
@@ -1,0 +1,155 @@
+import ConNF.Model.Result
+
+/-!
+# New file
+
+In this file...
+
+## Main declarations
+
+* `ConNF.foo`: Something new.
+-/
+
+noncomputable section
+universe u
+
+open Cardinal Ordinal ConNF.TSet
+
+namespace ConNF
+
+variable [Params.{u}] {α β γ δ ε ζ : Λ} (hβ : (β : TypeIndex) < α) (hγ : (γ : TypeIndex) < β)
+  (hδ : (δ : TypeIndex) < γ) (hε : (ε : TypeIndex) < δ) (hζ : (ζ : TypeIndex) < ε)
+
+def union (x y : TSet α) : TSet α :=
+  (xᶜ' ⊓' yᶜ')ᶜ'
+
+notation:68 x:68 " ⊔[" h "] " y:68 => _root_.ConNF.union h x y
+notation:68 x:68 " ⊔' " y:68 => x ⊔[by assumption] y
+
+@[simp]
+theorem mem_union_iff (x y : TSet α) :
+    ∀ z : TSet β, z ∈' x ⊔' y ↔ z ∈' x ∨ z ∈' y := by
+  rw [union]
+  intro z
+  rw [mem_compl_iff, mem_inter_iff, mem_compl_iff, mem_compl_iff, or_iff_not_and_not]
+
+def higherIndex (α : Λ) : Λ :=
+  (exists_gt α).choose
+
+theorem lt_higherIndex {α : Λ} :
+    (α : TypeIndex) < higherIndex α :=
+  WithBot.coe_lt_coe.mpr (exists_gt α).choose_spec
+
+theorem tSet_nonempty (h : ∃ β : Λ, (β : TypeIndex) < α) : Nonempty (TSet α) := by
+  obtain ⟨α', hα⟩ := h
+  constructor
+  apply typeLower lt_higherIndex lt_higherIndex lt_higherIndex hα
+  apply cardinalOne lt_higherIndex lt_higherIndex
+
+def univ : TSet α :=
+  (tSet_nonempty ⟨β, hβ⟩).some ⊔' (tSet_nonempty ⟨β, hβ⟩).someᶜ'
+
+@[simp]
+theorem mem_univ_iff :
+    ∀ x : TSet β, x ∈' univ hβ := by
+  intro x
+  rw [univ, mem_union_iff, mem_compl_iff]
+  exact em _
+
+/-- The set of all ordered pairs. -/
+def orderedPairs : TSet α :=
+  vCross hβ hγ hδ (univ hδ)
+
+@[simp]
+theorem mem_orderedPairs_iff (x : TSet β) :
+    x ∈' orderedPairs hβ hγ hδ ↔ ∃ a b, x = ⟨a, b⟩' := by
+  simp only [orderedPairs, vCross_spec, mem_univ_iff, and_true]
+
+def converse (x : TSet α) : TSet α :=
+  converse' hβ hγ hδ x ⊓' orderedPairs hβ hγ hδ
+
+@[simp]
+theorem op_mem_converse_iff (x : TSet α) :
+    ∀ a b, ⟨a, b⟩' ∈' converse hβ hγ hδ x ↔ ⟨b, a⟩' ∈' x := by
+  intro a b
+  simp only [converse, mem_inter_iff, converse'_spec, mem_orderedPairs_iff, op_inj, exists_and_left,
+    exists_eq', and_true]
+
+def cross (x y : TSet γ) : TSet α :=
+  converse hβ hγ hδ (vCross hβ hγ hδ x) ⊓' vCross hβ hγ hδ y
+
+@[simp]
+theorem mem_cross_iff (x y : TSet γ) :
+    ∀ a, a ∈' cross hβ hγ hδ x y ↔ ∃ b c, a = ⟨b, c⟩' ∧ b ∈' x ∧ c ∈' y := by
+  intro a
+  rw [cross, mem_inter_iff, vCross_spec]
+  constructor
+  · rintro ⟨h₁, b, c, rfl, h₂⟩
+    simp only [op_mem_converse_iff, vCross_spec, op_inj] at h₁
+    obtain ⟨b', c', ⟨rfl, rfl⟩, h₁⟩ := h₁
+    exact ⟨b, c, rfl, h₁, h₂⟩
+  · rintro ⟨b, c, rfl, h₁, h₂⟩
+    simp only [op_mem_converse_iff, vCross_spec, op_inj]
+    exact ⟨⟨c, b, ⟨rfl, rfl⟩, h₁⟩, ⟨b, c, ⟨rfl, rfl⟩, h₂⟩⟩
+
+def singletonImage (x : TSet β) : TSet α :=
+  singletonImage' hβ hγ hδ hε x ⊓' (cross hβ hγ hδ (cardinalOne hδ hε) (cardinalOne hδ hε))
+
+@[simp]
+theorem singletonImage_spec (x : TSet β) :
+    ∀ z w,
+    ⟨ {z}', {w}' ⟩' ∈' singletonImage hβ hγ hδ hε x ↔ ⟨z, w⟩' ∈' x := by
+  intro z w
+  rw [singletonImage, mem_inter_iff, singletonImage'_spec, and_iff_left_iff_imp]
+  intro hzw
+  rw [mem_cross_iff]
+  refine ⟨{z}', {w}', rfl, ?_⟩
+  simp only [mem_cardinalOne_iff, singleton_inj, exists_eq', and_self]
+
+theorem exists_of_mem_singletonImage {x : TSet β} {z w : TSet δ}
+    (h : ⟨z, w⟩' ∈' singletonImage hβ hγ hδ hε x) :
+    ∃ a b, z = {a}' ∧ w = {b}' := by
+  simp only [singletonImage, mem_inter_iff, mem_cross_iff, op_inj, mem_cardinalOne_iff] at h
+  obtain ⟨-, _, _, ⟨rfl, rfl⟩, ⟨a, rfl⟩, ⟨b, rfl⟩⟩ := h
+  exact ⟨a, b, rfl, rfl⟩
+
+/-- Turn a model element encoding a relation into an actual relation. -/
+def ExternalRel (r : TSet α) : Rel (TSet δ) (TSet δ) :=
+  λ x y ↦ ⟨x, y⟩' ∈' r
+
+@[simp]
+theorem externalRel_converse (r : TSet α) :
+    ExternalRel hβ hγ hδ (converse hβ hγ hδ r) = (ExternalRel hβ hγ hδ r).inv := by
+  ext
+  simp only [ExternalRel, op_mem_converse_iff, Rel.inv_apply]
+
+/-- The codomain of a relation. -/
+def codom (r : TSet α) : TSet γ :=
+  (typeLower lt_higherIndex hβ hγ hδ (singletonImage lt_higherIndex hβ hγ hδ r)ᶜ[lt_higherIndex])ᶜ'
+
+@[simp]
+theorem mem_codom_iff (r : TSet α) (x : TSet δ) :
+    x ∈' codom hβ hγ hδ r ↔ x ∈ (ExternalRel hβ hγ hδ r).codom := by
+  simp only [codom, mem_compl_iff, mem_typeLower_iff, not_forall, not_not]
+  constructor
+  · rintro ⟨y, hy⟩
+    obtain ⟨a, b, rfl, hb⟩ := exists_of_mem_singletonImage lt_higherIndex hβ hγ hδ hy
+    rw [singleton_inj] at hb
+    subst hb
+    rw [singletonImage_spec] at hy
+    exact ⟨a, hy⟩
+  · rintro ⟨a, ha⟩
+    use {a}'
+    rw [singletonImage_spec]
+    exact ha
+
+/-- The domain of a relation. -/
+def dom (r : TSet α) : TSet γ :=
+  codom hβ hγ hδ (converse hβ hγ hδ r)
+
+@[simp]
+theorem mem_dom_iff (r : TSet α) (x : TSet δ) :
+    x ∈' dom hβ hγ hδ r ↔ x ∈ (ExternalRel hβ hγ hδ r).dom := by
+  rw [dom, mem_codom_iff, externalRel_converse, Rel.inv_codom]
+
+end ConNF
