ConNF/External/WellOrder.lean
@@ -1,0 +1,31 @@
+import ConNF.External.Basic
+
+/-!
+# New file
+
+In this file...
+
+## Main declarations
+
+* `ConNF.foo`: Something new.
+-/
+
+noncomputable section
+universe u
+
+open Cardinal Ordinal ConNF.TSet
+
+namespace ConNF
+
+variable [Params.{u}] {α β γ δ ε ζ : Λ} (hβ : (β : TypeIndex) < α) (hγ : (γ : TypeIndex) < β)
+  (hδ : (δ : TypeIndex) < γ) (hε : (ε : TypeIndex) < δ) (hζ : (ζ : TypeIndex) < ε)
+
+/-- A set in our model that is a well-order. Internal well-orders are exactly external well-orders,
+so we externalise the definition for convenience. -/
+def InternalWellOrder (r : TSet α) : Prop :=
+  IsWellOrder (TSet δ) (ExternalRel hβ hγ hδ r)
+
+def InternallyWellOrdered (x : TSet γ) : Prop :=
+  ∃ r, InternalWellOrder hβ hγ hδ r ∧ x = dom hβ hγ hδ r
+
+end ConNF
