ConNF/Levels/StrSet.lean
@@ -132,7 +132,8 @@ end StrSet
 class TypedMem (X Y : Type _) (β α : outParam TypeIndex) where
   typedMem : β < α → X → Y → Prop
 
-notation:50 x:50 " ∈[" h:50 "] " y:50 => TypedMem.typedMem h x y
+notation:50 x:50 " ∈[" h "] " y:50 => TypedMem.typedMem h x y
+notation:50 x:50 " ∈' " y:50 => TypedMem.typedMem (by assumption) x y
 
 instance {β α : TypeIndex} : TypedMem (StrSet β) (StrSet α) β α where
   typedMem h x y :=
